feat: add properties to Regex.Captures

Regex/Regex.lean
@@ -5,6 +5,7 @@ import Regex.Backtrack
 import Regex.Utils
 import Regex.Syntax.Ast.Parser
 import Regex.Syntax.Translate
+import Regex.Data.Array.Basic
 
 open NFA
 
@@ -34,24 +35,28 @@ instance : ToString Match where
   toString s :=
     s!"'{s}', {s.startPos}, {s.stopPos}"
 
-/-- Represents the capture groups for a single match. -/
-structure Captures where
+/-- Represents the full match and capture groups for a single match in `s`. -/
+structure Captures (s : String) where
   /-- the full match -/
   fullMatch : Match
   /-- the capture groups -/
   groups: Array (Option Match)
+  /-- `fullMatch` is a substring of `s`. -/
+  isSubstringOf : fullMatch.str = s
+  /-- all matches in `groups` are substrings of `s`. -/
+  areSubstringsOf : groups.all (Option.all (·.str = s) ·)
 
 namespace Captures
 
-def end? (c : Captures) : Option String.Pos :=
+def end? (c : Captures s) : Option String.Pos :=
   c.fullMatch.stopPos
 
-def «matches» (c : Captures) :Array (Option Match) :=
+def «matches» (c : Captures s) :Array (Option Match) :=
   #[(some c.fullMatch)] ++ c.groups
 
 end Captures
 
-instance : ToString Captures where
+instance : ToString (Captures s) where
   toString c := s!"fullMatch: {c.fullMatch}\ngroups: {c.groups}"
 
 /-- Build a Regex from the given pattern. -/
@@ -59,7 +64,8 @@ def build (s : String) (flavor : Syntax.Flavor := default)
     (flags : Syntax.Flags := default) (config : Compiler.Config := default)
     (extended : Regex.Grammar.ExtendedKind := .None)
     : Except String Regex := do
-  let nfa ← Syntax.AstItems.parse s flavor extended >>= Syntax.translate flags >>= Compiler.compile config
+  let nfa ← Syntax.AstItems.parse s flavor extended
+              >>= Syntax.translate flags >>= Compiler.compile config
   Except.ok ⟨nfa⟩
 
 namespace Log
@@ -67,23 +73,19 @@ namespace Log
 /-- This routine searches for the first match of this regex in the haystack given,
     returns an array of log msgs, the overall match and the matches of each capture group -/
 def captures (s : Substring) (re : Regex) («at» : String.Pos) (logEnabled : Bool)
-    : Array String × Option Captures :=
-  let (msgs, slots) := BoundedBacktracker.slots s «at» re.nfa logEnabled
-  let «matches» : Array (Option Match) := slots
-            |> Array.map (fun pair =>
-                match pair with
-                | some (p0, p1) => some ⟨s.str, p0, p1⟩
-                | none => none)
-
+    : Array String × Option (Captures s.str) :=
+  let (msgs, «matches») := BoundedBacktracker.«matches» s «at» re.nfa logEnabled
   match «matches».head? with
-  | some (some head, tail) => (msgs, some ⟨head, tail⟩)
+  | some (some head, tail) =>
+    let tail := tail.map_option_subtype
+    (msgs, some ⟨head.val, tail.val, head.property, tail.property⟩)
   | _ => (msgs, none)
 
-private def is_overlapping_empty_match (start «end» : String.Pos) (acc : Array Captures) : Bool :=
+private def is_overlapping_empty_match (f t : String.Pos) (acc : Array (Captures s)) : Bool :=
   match acc.pop? with
   | some (last, _) =>
       match last.end? with
-      | some previous_end => start = «end» && previous_end = «end»
+      | some previous_end => f = t && previous_end = t
       | none => false
   | none => false
 
@@ -101,7 +103,8 @@ theorem String.Pos.sizeof_lt_of_lt {a b : String.Pos} (h : a < b) : sizeOf a < s
   omega
 
 private def all_captures_loop (s : Substring) («at» : String.Pos) (re : Regex)
-    (logEnabled : Bool) (acc : Array String × Array Captures) : Array String × Array Captures :=
+  (logEnabled : Bool) (acc : Array String × Array (Captures s.str))
+    : Array String × Array (Captures s.str) :=
   match Log.captures s re «at» logEnabled with
   | (msgs, some captures) =>
     let  ⟨_, start, «end»⟩ := captures.fullMatch
@@ -122,7 +125,7 @@ termination_by s.stopPos - «at»
 
 /-- Returns an array of log msgs and all successive non-overlapping matches in the given haystack. -/
 def all_captures (s : Substring) (re : Regex) (logEnabled : Bool)
-    : Array String × Array Captures :=
+    : Array String × Array (Captures s.str) :=
   all_captures_loop s ⟨0⟩ re logEnabled (#[], #[])
 
 end Log
@@ -130,11 +133,11 @@ end Log
 /-- This routine searches for the first match of this regex in the haystack given, and if found,
     returns not only the overall match but also the matches of each capture group in the regex.
     If no match is found, then None is returned. -/
-def captures (s : Substring) (re : Regex) («at» : String.Pos := ⟨0⟩) : Option Captures :=
+def captures (s : Substring) (re : Regex) («at» : String.Pos := ⟨0⟩) : Option (Captures s.str) :=
   let (_, captures) := Log.captures s re «at» false
   captures
 
 /-- Returns all successive non-overlapping matches in the given haystack. -/
-def all_captures (s : Substring) (re : Regex) : Array Captures :=
+def all_captures (s : Substring) (re : Regex) : Array (Captures s.str) :=
   let (_, captures) := Log.all_captures s re false
   captures
