Regex/Data/Array/Basic.lean
@@ -29,3 +29,34 @@ def unique [BEq α] (intervals: Array α) : Array α :=
         if prev == r then (r, unique)
         else (r, unique.push r))
     unique
+
+/-- Unattach values of subtype in `arr` and collect their properties. -/
+def map_option_subtype {p : α → Prop} [DecidablePred p] (arr : Array (Option { m : α // p m }))
+    : { arr : Array (Option α) // arr.all (Option.all (p · ) ·) } :=
+  ⟨arr.map (Option.map (·.val)), by
+    cases arr
+    rename_i l
+    induction l with
+    | nil => rfl
+    | cons a l ih =>
+        rw [Array.all_eq_true_iff_forall_mem] at ih
+        rw [Array.all_eq_true_iff_forall_mem]
+        intros x h
+        match x with
+        | none => rfl
+        | some x =>
+          unfold Option.all
+          split <;> try simp_all
+          rename_i val heq
+          cases h
+          · rename_i h
+            simp [Option.unattach, -Option.map_subtype] at h
+            unfold Option.map at h
+            split at h <;> try simp_all
+            rename_i x
+            exact x.property
+          · rename_i h
+            let ⟨x, hx⟩ := h
+            have h := ih x hx.left
+            rw [hx.right] at h
+            simp_all⟩
